theories/examples/run_yield_with_unknown/ftlr.v
@@ -2,8 +2,7 @@ From iris.proofmode Require Import tactics.
 From machine_program_logic.program_logic Require Import weakestpre.
 From HypVeri.lang Require Import lang.
 From HypVeri.algebra Require Import base base_extra.
-(* From HypVeri.rules Require Import rules_base (* nop mov ldr str halt fail add sub mult cmp *). *)
-From HypVeri.logrel Require Import logrel logrel_extra.
+From HypVeri.logrel Require Import logrel logrel_extra fundamental.
 From HypVeri Require Import proofmode.
 From HypVeri.examples Require Import run_yield_with_unknown.proof.
 Import uPred.
@@ -12,11 +11,12 @@ Section rywu_ftlr.
   Context `{hypparams:!HypervisorParameters}.
   Context `{vmG: !gen_VMG Σ}.
 
-  Definition rywu_interp_access (p_prog3 p_tx p_rx :PID):= interp_access V2 {[p_prog3]} p_tx p_rx ∅.
+  Definition rywu_interp_access (p_prog3 p_tx p_rx :PID):= interp_access V2 {[p_prog3;p_tx;p_rx]} p_tx p_rx ∅.
 
   Lemma rywu_ftlr (p_prog3 p_tx p_rx :PID):
    rywu_interp_access p_prog3 p_tx p_rx ⊢ interp_execute V2.
   Proof.
-  Admitted.
+    iApply ftlr.
+  Qed.
 
 End rywu_ftlr.
