theories/rules/rules_base.v
@@ -85,7 +85,7 @@ Proof.
   rewrite /scheduled /machine.scheduler //= /scheduler.
 Qed.
 
-
+(* TODO: we don't necessarily need full acc *)
 Lemma not_valid_pc {s} i a :
   (tpa a) ∉ s ->
   {SS{{ ▷ (PC @@ i ->r a) ∗ ▷ i -@A> [s] }}}
@@ -138,19 +138,20 @@ Proof.
       inversion H.
 Qed.
 
-Lemma not_valid_instr {q} i a wi :
+Lemma not_valid_instr {q s} i a wi :
   decode_instruction wi = None ->
+  (tpa a) ∈ s ->
   {SS{{ ▷ (PC @@ i ->r a)
-        ∗ ▷ i -@{q}A> (tpa a)
+        ∗ ▷ i -@{q}A> [s]
         ∗ ▷ a ->a wi}}}
   ExecI @ i
   {{{ RET (false, FailI);
     PC @@ i ->r a
-    ∗ i -@{q}A> (tpa a)
+    ∗ i -@{q}A> [s]
     ∗ a ->a wi
   }}}.
 Proof.
-  iIntros (Hdecode_none ϕ) "(>Hpc & >Ha & >Hw) Hϕ".
+  iIntros (Hdecode_none Hin ϕ) "(>Hpc & >Ha & >Hw) Hϕ".
   iApply (sswp_lift_atomic_step ExecI);[done|].
   iIntros (n σ1) "%Hsche Hσ1".
   rewrite /scheduled /= /scheduler /Is_true in Hsche.
@@ -161,8 +162,7 @@ Proof.
   iModIntro.
   iDestruct "Hσ1" as "( ? & Hmem & Hreg & ? & ? & ? & Haccess & ?)".
   iDestruct (gen_reg_valid1 PC i a Hcur with "Hreg Hpc") as "%Hpc".
-  iDestruct (access_agree_check_true (tpa a) i with "Haccess Ha") as "%Hacc".
-  { set_solver +. }
+  iDestruct (access_agree_check_true (tpa a) i with "Haccess Ha") as "%Hacc";first auto.
   iDestruct (gen_mem_valid with "Hmem Hw") as "%Hlookup_w".
   iSplit.
   - iPureIntro.
